Rest of the previous refinement adequacy proof (after fixing the statement).

src/CSL/Refinement.v
@@ -28,15 +28,19 @@ Context {Λ: Layer OpT}.
 Definition tpoolUR := gmapUR nat (exclR (procTC OpT)).
 Definition stateUR := optionUR (exclR (StateC _ Λ)).
 Definition cfgUR := prodUR tpoolUR stateUR.
+
+Class cfgPreG (Σ : gFunctors) :=
+  { cfg_preG_inG :> inG Σ (authR cfgUR) }.
 Class cfgG Σ := { cfg_inG :> inG Σ (authR cfgUR); cfg_name : gname }.
 
-Fixpoint tpool_to_map_aux (tp: thread_pool OpT) (id: nat) : tpoolUR :=
+Fixpoint tpool_to_map_aux (tp: thread_pool OpT) (id: nat) : gmap nat (@procT OpT):=
   match tp with
   | [] => ∅
-  | e :: tp' => <[id := Excl e]>(tpool_to_map_aux tp' (S id))
+  | e :: tp' => <[id := e]>(tpool_to_map_aux tp' (S id))
   end.
 
 Definition tpool_to_map tp := tpool_to_map_aux tp O.
+Definition tpool_to_res tp := (Excl <$> (tpool_to_map tp) : tpoolUR).
 
 Definition sourceN := nroot .@ "source".
 
@@ -48,7 +52,7 @@ Section ghost_spec.
 
   (* ownership of this does not mean there aren't other threads not in (fst ρ) *)
   Definition source_cfg ρ : iProp Σ :=
-    own cfg_name (◯ (tpool_to_map (fst ρ), Some (Excl (snd ρ)))).
+    own cfg_name (◯ (tpool_to_res (fst ρ), Some (Excl (snd ρ)))).
 
   Definition source_state (σ: State Λ) : iProp Σ :=
     own cfg_name (◯ (∅ : tpoolUR, Some (Excl σ))).
@@ -57,7 +61,7 @@ Section ghost_spec.
     own cfg_name (◯ (Excl <$> tp : gmap nat (exclR (procTC OpT)), ε)).
 
   Definition source_inv (tp: thread_pool OpT) (σ: State Λ) : iProp Σ :=
-    (∃ tp' σ', own cfg_name (● (tpool_to_map tp', Some (Excl σ')))  ∗
+    (∃ tp' σ', own cfg_name (● (tpool_to_res tp', Some (Excl σ')))  ∗
                  ⌜ bind_star (exec_pool Λ) tp σ σ' tp' ⌝)%I.
 
   Definition source_ctx ρ : iProp Σ :=
@@ -75,16 +79,14 @@ End ghost_spec.
 Notation "j ⤇ e" := (tpool_mapsto j e) (at level 20) : bi_scope.
 
 Section ghost_step.
-  Context `{cfgG Σ, invG Σ}.
-  Context `{Inhabited Λ.(State)}.
+  Context `{invG Σ}.
 
   Lemma tpool_to_map_lookup_aux tp id j e:
-    tpool_to_map_aux tp id !! (id + j) = Some (Excl e) ↔ tp !! j = Some e.
+    tpool_to_map_aux tp id !! (id + j) = Some e ↔ tp !! j = Some e.
   Proof.
     revert id j; induction tp => id j //=.
     destruct j.
     * rewrite //= Nat.add_0_r lookup_insert //=.
-      split; inversion 1; auto; setoid_subst; eauto.
     * rewrite //= lookup_insert_ne //=; last by lia.
       replace (id + S j) with (S id + j) by lia; eauto.
   Qed.
@@ -100,7 +102,7 @@ Section ghost_step.
   Qed.
 
   Lemma tpool_to_map_lookup tp j e:
-    tpool_to_map tp !! j = Some (Excl e) ↔ tp !! j = Some e.
+    tpool_to_map tp !! j = Some e ↔ tp !! j = Some e.
   Proof.
     rewrite /tpool_to_map. pose (tpool_to_map_lookup_aux tp 0 j e) => //=.
   Qed.
@@ -111,91 +113,144 @@ Section ghost_step.
     rewrite /tpool_to_map. pose (tpool_to_map_lookup_aux_none tp 0 j) => //=.
   Qed.
 
-  Lemma tpool_to_map_lookup_excl tp j x:
-    tpool_to_map tp !! j = Some x → ∃ e, x = Excl e.
+  Lemma tpool_to_res_lookup tp j e:
+    tpool_to_res tp !! j = Some (Excl e) ↔ tp !! j = Some e.
   Proof.
-    rewrite /tpool_to_map. generalize 0. induction tp => n //=.
-    destruct (decide (j = n)); subst.
-    * rewrite lookup_insert. inversion 1; setoid_subst; by eexists.
-    * rewrite lookup_insert_ne //=; eauto.
+    rewrite /tpool_to_res lookup_fmap. generalize (tpool_to_map_lookup tp j e) => Hconv.
+    split.
+    - destruct (tpool_to_map tp !! j); inversion 1; subst; eapply Hconv; eauto.
+    - intros. rewrite (proj2 Hconv); eauto.
   Qed.
 
-  Lemma tpool_to_map_insert_update tp j e :
+  Lemma tpool_to_res_lookup_none tp j:
+    tpool_to_res tp !! j = None ↔ tp !! j = None.
+  Proof.
+    rewrite /tpool_to_res lookup_fmap. generalize (tpool_to_map_lookup_none tp j) => Hconv.
+    split.
+    -destruct (tpool_to_map tp !! j); inversion 1; subst; eapply Hconv; eauto.
+    - intros. rewrite (proj2 Hconv); eauto.
+  Qed.
+
+  Lemma tpool_to_res_lookup_excl tp j x:
+    tpool_to_res tp !! j = Some x → ∃ e, x = Excl e.
+  Proof.
+    rewrite /tpool_to_res/tpool_to_map. generalize 0. induction tp => n //=.
+    destruct (decide (j = n)); subst.
+    * rewrite lookup_fmap //= lookup_insert. inversion 1; setoid_subst; by eexists.
+    * rewrite lookup_fmap //= lookup_insert_ne //= -lookup_fmap; eauto.
+  Qed.
+
+  Lemma tpool_to_res_insert_update tp j e :
     j < length tp →
-    tpool_to_map (<[j := e]> tp) = <[j := Excl e]> (tpool_to_map tp).
+    tpool_to_res (<[j := e]> tp) = <[j := Excl e]> (tpool_to_res tp).
   Proof.
     intros Hlt. apply: map_eq; intros i.
     destruct (decide (i = j)); subst.
-    - rewrite lookup_insert tpool_to_map_lookup list_lookup_insert //=.
+    - rewrite lookup_insert tpool_to_res_lookup list_lookup_insert //=.
     - rewrite lookup_insert_ne //=.
       destruct (decide (i < length tp)) as [Hl|Hnl].
       * efeed pose proof (lookup_lt_is_Some_2 tp) as His; first eassumption.
         destruct His as (e'&His).
-        rewrite (proj2 (tpool_to_map_lookup tp i e')) //=.
-        apply tpool_to_map_lookup. rewrite list_lookup_insert_ne //=.
+        rewrite (proj2 (tpool_to_res_lookup tp i e')) //=.
+        apply tpool_to_res_lookup. rewrite list_lookup_insert_ne //=.
       * efeed pose proof (lookup_ge_None_2 tp i) as Hnone; first lia.
-        rewrite (proj2 (tpool_to_map_lookup_none tp i)) //=.
-        apply tpool_to_map_lookup_none. rewrite list_lookup_insert_ne //=.
+        rewrite (proj2 (tpool_to_res_lookup_none tp i)) //=.
+        apply tpool_to_res_lookup_none. rewrite list_lookup_insert_ne //=.
   Qed.
 
-  Lemma tpool_to_map_insert_snoc tp e :
-    tpool_to_map (tp ++ [e]) = <[length tp := Excl e]> (tpool_to_map tp).
+  Lemma tpool_to_res_insert_snoc tp e :
+    tpool_to_res (tp ++ [e]) = <[length tp := Excl e]> (tpool_to_res tp).
   Proof.
     apply: map_eq; intros i.
     destruct (decide (i = length tp)); subst.
-    - rewrite lookup_insert tpool_to_map_lookup.
+    - rewrite lookup_insert tpool_to_res_lookup.
       rewrite lookup_app_r //= Nat.sub_diag //=.
     - rewrite lookup_insert_ne //=.
       destruct (decide (i < length tp)) as [Hl|Hnl].
       * efeed pose proof (lookup_lt_is_Some_2 tp) as His; first eassumption.
         destruct His as (e'&His).
-        rewrite (proj2 (tpool_to_map_lookup tp i e')) //=.
-        apply tpool_to_map_lookup. rewrite lookup_app_l //=.
+        rewrite (proj2 (tpool_to_res_lookup tp i e')) //=.
+        apply tpool_to_res_lookup. rewrite lookup_app_l //=.
       * efeed pose proof (lookup_ge_None_2 tp i) as Hnone; first lia.
-        rewrite (proj2 (tpool_to_map_lookup_none tp i)) //=.
-        apply tpool_to_map_lookup_none. rewrite lookup_ge_None_2 //= app_length //=; lia.
+        rewrite (proj2 (tpool_to_res_lookup_none tp i)) //=.
+        apply tpool_to_res_lookup_none. rewrite lookup_ge_None_2 //= app_length //=; lia.
   Qed.
 
-  Lemma tpool_to_map_length tp j e :
-    tpool_to_map tp !! j = Some e → j < length tp.
+  Lemma tpool_to_res_length tp j e :
+    tpool_to_res tp !! j = Some e → j < length tp.
   Proof.
     intros Hlookup. destruct (decide (j < length tp)) as [Hl|Hnl]; auto.
-    rewrite (proj2 (tpool_to_map_lookup_none tp j)) in Hlookup; first by congruence.
+    rewrite (proj2 (tpool_to_res_lookup_none tp j)) in Hlookup; first by congruence.
     apply lookup_ge_None_2; lia.
   Qed.
 
   Lemma tpool_singleton_included1 tp j e :
-    {[j := Excl e]} ≼ tpool_to_map tp → tpool_to_map tp !! j = Some (Excl e).
+    {[j := Excl e]} ≼ tpool_to_res tp → tpool_to_res tp !! j = Some (Excl e).
   Proof.
     intros (x&Hlookup&Hexcl)%singleton_included.
-    destruct (tpool_to_map_lookup_excl tp j x) as (e'&Heq); setoid_subst; eauto.
+    destruct (tpool_to_res_lookup_excl tp j x) as (e'&Heq); setoid_subst; eauto.
     apply Excl_included in Hexcl; setoid_subst; auto.
   Qed.
 
   Lemma tpool_singleton_included2 tp j e :
-    {[j := Excl e]} ≼ tpool_to_map tp → tp !! j = Some e.
+    {[j := Excl e]} ≼ tpool_to_res tp → tp !! j = Some e.
   Proof.
     intros Hlookup%tpool_singleton_included1.
-    apply tpool_to_map_lookup; rewrite Hlookup; eauto.
+    apply tpool_to_res_lookup; rewrite Hlookup; eauto.
   Qed.
 
   Lemma tpool_map_included1 tp1 tp2 :
-    Excl <$> tp1 ≼ tpool_to_map tp2 → (∀ j e, tp1 !! j = Some e → tp2 !! j = Some e).
+    Excl <$> tp1 ≼ tpool_to_res tp2 → (∀ j e, tp1 !! j = Some e → tp2 !! j = Some e).
   Proof.
     rewrite lookup_included => Hincl j e Hin.
-    specialize (Hincl j). apply tpool_to_map_lookup.
+    specialize (Hincl j). apply tpool_to_res_lookup.
     rewrite (lookup_fmap _ tp1 j) Hin //= in Hincl.
-    destruct (tpool_to_map tp2 !! j) as [x|] eqn: Heq; rewrite Heq in Hincl.
+    destruct (tpool_to_res tp2 !! j) as [x|] eqn: Heq; rewrite Heq in Hincl.
     {
-      destruct (tpool_to_map_lookup_excl tp2 j x) as (e'&Heq'); setoid_subst; eauto.
+      destruct (tpool_to_res_lookup_excl tp2 j x) as (e'&Heq'); setoid_subst; eauto.
       apply Excl_included in Hincl; setoid_subst; eauto.
     }
     apply option_included in Hincl as [Hfalse|(?&?&?&?&?)]; congruence.
   Qed.
 
+  Lemma tpool_to_res_lookup_case tp j:
+    (tpool_to_res tp !! j = None) ∨ (∃ e, tpool_to_res tp !! j = Excl' e).
+  Proof.
+    rewrite /tpool_to_res.
+    destruct (tpool_to_map tp !! j) as [p|] eqn:Heq; rewrite lookup_fmap Heq //=.
+    * by (right; exists p).
+    * by left.
+  Qed.
+
+  Lemma source_cfg_init `{cfgPreG Σ} tp σ :
+    (|={⊤}=> ∃ _ : cfgG Σ, source_ctx (tp, σ) ∗ source_pool_map (tpool_to_map tp) ∗ source_state σ)%I.
+  Proof.
+    iMod (own_alloc (● (tpool_to_res tp, Some (Excl σ))
+                       ⋅ ◯ (tpool_to_res tp, Some (Excl σ)))) as (γ) "(Hauth&Hfrag)".
+    { apply @auth_valid_discrete_2; first by apply _. split; [| split].
+      { reflexivity. }
+      - rewrite //=. intros i.
+        destruct (tpool_to_res_lookup_case tp i) as [Heq_none|(e&Heq_some)].
+        * rewrite Heq_none; econstructor.
+        * rewrite Heq_some; econstructor.
+      - rewrite //=.
+    }
+    set (IN := {| cfg_name := γ |}).
+    iExists IN.
+    iMod (inv_alloc sourceN ⊤ (source_inv tp σ) with "[Hauth]").
+    { rewrite /source_inv. iNext. iExists tp, σ. iFrame "Hauth".
+      iPureIntro; econstructor. }
+    iModIntro. iFrame.
+    rewrite pair_split.
+    iDestruct "Hfrag" as "($&$)".
+  Qed.
+
+  Context `{cfgG Σ}.
+  Context `{Inhabited Λ.(State)}.
+
   Lemma source_thread_update {T T'} (e': proc OpT T') tp j (e: proc OpT T)  σ :
-    j ⤇ e -∗ own cfg_name (● (tpool_to_map tp, Excl' σ))
-      ==∗ j ⤇ e' ∗ own cfg_name (● (tpool_to_map (<[j := existT _ e']>tp), Excl' σ)).
+    j ⤇ e -∗ own cfg_name (● (tpool_to_res tp, Excl' σ))
+      ==∗ j ⤇ e' ∗ own cfg_name (● (tpool_to_res (<[j := existT _ e']>tp), Excl' σ)).
   Proof.
     iIntros "Hj Hauth".
     iDestruct (own_valid_2 with "Hauth Hj") as %Hval_pool.
@@ -209,22 +264,22 @@ Section ghost_step.
       { econstructor. }
     }
     iFrame.
-    rewrite tpool_to_map_insert_update //; last first.
-    { eapply tpool_to_map_length; eauto. }
+    rewrite tpool_to_res_insert_update //; last first.
+    { eapply tpool_to_res_length; eauto. }
   Qed.
 
   Lemma source_threads_fork (efs: thread_pool OpT) tp σ :
-    own cfg_name (● (tpool_to_map tp, Excl' σ))
+    own cfg_name (● (tpool_to_res tp, Excl' σ))
       ==∗ ([∗ list] ef ∈ efs, ∃ j', j' ⤇ `(projT2 ef))
-        ∗ own cfg_name (● (tpool_to_map (tp ++ efs), Excl' σ)).
+        ∗ own cfg_name (● (tpool_to_res (tp ++ efs), Excl' σ)).
   Proof.
     iInduction efs as [| ef efs] "IH" forall (tp).
     - rewrite /= app_nil_r /=; auto.
     - iIntros "Hown".
       iMod (own_update with "Hown") as "[Hown Hj']".
       eapply auth_update_alloc, prod_local_update_1.
-      eapply (alloc_local_update (tpool_to_map tp) _ (length tp) (Excl ef)).
-      { apply tpool_to_map_lookup_none, lookup_ge_None_2. reflexivity. }
+      eapply (alloc_local_update (tpool_to_res tp) _ (length tp) (Excl ef)).
+      { apply tpool_to_res_lookup_none, lookup_ge_None_2. reflexivity. }
       { econstructor. }
       iEval (rewrite insert_empty) in "Hj'".
       rewrite //= -assoc.
@@ -232,12 +287,12 @@ Section ghost_step.
       { iExists (length tp); destruct ef; iModIntro; eauto. }
       replace (ef :: efs) with ([ef] ++ efs) by auto.
       rewrite assoc. iApply "IH".
-      rewrite tpool_to_map_insert_snoc; eauto.
+      rewrite tpool_to_res_insert_snoc; eauto.
   Qed.
 
   Lemma source_state_update σ' tp σ1 σ2 :
-    source_state σ1 -∗ own cfg_name (● (tpool_to_map tp, Excl' σ2))
-      ==∗ source_state σ' ∗ own cfg_name (● (tpool_to_map tp, Excl' σ')).
+    source_state σ1 -∗ own cfg_name (● (tpool_to_res tp, Excl' σ2))
+      ==∗ source_state σ' ∗ own cfg_name (● (tpool_to_res tp, Excl' σ')).
   Proof.
     iIntros "Hstate Hauth".
     iDestruct (own_valid_2 with "Hauth Hstate") as %Hval_state.
@@ -252,16 +307,16 @@ Section ghost_step.
   Qed.
 
   Lemma source_thread_reconcile {T} tp j e x:
-    j ⤇ e -∗ own cfg_name (● (tpool_to_map tp, x)) -∗ ⌜ tp !! j = Some (existT T e) ⌝.
+    j ⤇ e -∗ own cfg_name (● (tpool_to_res tp, x)) -∗ ⌜ tp !! j = Some (existT T e) ⌝.
   Proof.
     iIntros "Hj Hauth".
     iDestruct (own_valid_2 with "Hauth Hj") as %Hval_pool.
     apply auth_valid_discrete_2 in Hval_pool as ((Hpool&_)%prod_included&Hval').
-    apply tpool_singleton_included1, tpool_to_map_lookup in Hpool; eauto.
+    apply tpool_singleton_included1, tpool_to_res_lookup in Hpool; eauto.
   Qed.
 
   Lemma source_pool_map_reconcile tp1 tp2 x:
-    source_pool_map tp1 -∗ own cfg_name (● (tpool_to_map tp2, x)) -∗
+    source_pool_map tp1 -∗ own cfg_name (● (tpool_to_res tp2, x)) -∗
                     ⌜ ∀ i e, tp1 !! i = Some e → tp2 !! i = Some e ⌝.
   Proof.
     iIntros "Hj Hauth".
